spot/GC.SPOT.ConcreteFull.fst
@@ -59,7 +59,7 @@ let post_roots_mem_c
           (ConcreteMajor.spot_major_heap r)
           (ConcreteMajor.spot_major_fp r)
           (ThreeObjects.spot_roots (ConcreteMajor.spot_c r))
-          roots_out st cap)
+          roots_out true st cap)
       (ensures
         Seq.mem (ConcreteMajor.spot_c r <: U64.t) roots_out /\
         Seq.mem (ConcreteMajor.spot_c r)
@@ -118,7 +118,7 @@ let post_roots_mem_a_prime
           (ConcreteMajor.spot_major_heap r)
           (ConcreteMajor.spot_major_fp r)
           (ThreeObjects.spot_roots (ConcreteMajor.spot_c r))
-          roots_out st cap)
+          roots_out true st cap)
       (ensures (
         let prom = Cheney.cheney_promote
           ConcreteMinor.spot_minor2
@@ -188,7 +188,8 @@ let root_heap_reachable_from_major_gc_pre
       (requires
         GenInv.collection_heap_shape minor major fp /\
         MinorFwd.roots_valid_for_minor_collection minor major roots /\
-        GenImpl.gen_gc_major_precondition minor major fp roots st cap /\
+        CheneyBFS.cheney_no_oom minor major fp roots /\
+        GenImpl.gen_gc_stack_budget roots st cap /\
         Seq.mem r (GenImpl.gen_gc_prepared_roots minor major fp roots st cap))
       (ensures
         SpecCorrectness.heap_reachable
@@ -218,10 +219,7 @@ let spot_root_heap_reachable_from_major_gc_pre
   : Lemma
       (requires (
         let roots = ThreeObjects.spot_roots (ConcreteMajor.spot_c r) in
-        GenImpl.gen_gc_major_precondition
-          ConcreteMinor.spot_minor2
-          (ConcreteMajor.spot_major_heap r)
-          (ConcreteMajor.spot_major_fp r) roots st cap /\
+        GenImpl.gen_gc_stack_budget roots st cap /\
         Seq.mem v (GenImpl.gen_gc_prepared_roots
           ConcreteMinor.spot_minor2
           (ConcreteMajor.spot_major_heap r)
@@ -241,6 +239,7 @@ let spot_root_heap_reachable_from_major_gc_pre
   =
   ConcreteScenarios.spot_collection_heap_shape r;
   ConcreteScenarios.spot_roots_valid_for_minor_collection r;
+  ConcreteForwarding.spot_concrete_no_oom r;
   root_heap_reachable_from_major_gc_pre
     ConcreteMinor.spot_minor2
     (ConcreteMajor.spot_major_heap r)
@@ -270,12 +269,7 @@ let spot_concrete_c_final_survives
       (ConcreteMajor.spot_major_fp r)
       (ThreeObjects.spot_roots c)
       st cap));
-  assert (GenImpl.gen_gc_major_precondition
-    ConcreteMinor.spot_minor2
-    (ConcreteMajor.spot_major_heap r)
-    (ConcreteMajor.spot_major_fp r)
-    (ThreeObjects.spot_roots c)
-    st cap);
+  assert (GenImpl.gen_gc_stack_budget (ThreeObjects.spot_roots c) st cap);
   spot_root_heap_reachable_from_major_gc_pre r st cap c;
   ThreeObjects.spot_final_survives_from_gen_gc_post
     ConcreteMinor.spot_minor2
@@ -313,12 +307,7 @@ let spot_concrete_a_prime_final_survives
       (ConcreteMajor.spot_major_fp r)
       (ThreeObjects.spot_roots c)
       st cap));
-  assert (GenImpl.gen_gc_major_precondition
-    ConcreteMinor.spot_minor2
-    (ConcreteMajor.spot_major_heap r)
-    (ConcreteMajor.spot_major_fp r)
-    (ThreeObjects.spot_roots c)
-    st cap);
+  assert (GenImpl.gen_gc_stack_budget (ThreeObjects.spot_roots c) st cap);
   spot_root_heap_reachable_from_major_gc_pre r st cap a_prime;
   ThreeObjects.spot_final_survives_from_gen_gc_post
     ConcreteMinor.spot_minor2
@@ -415,7 +404,7 @@ let post_roots_shape
           (ConcreteMajor.spot_major_heap r)
           (ConcreteMajor.spot_major_fp r)
           (ThreeObjects.spot_roots (ConcreteMajor.spot_c r))
-          roots_out st cap)
+          roots_out true st cap)
       (ensures (
         let c = ConcreteMajor.spot_c r in
         let prom = Cheney.cheney_promote
@@ -513,11 +502,8 @@ let prepared_roots_preserve_c_field1
           (ConcreteMajor.spot_major_heap r)
           (ConcreteMajor.spot_major_fp r)
           (ThreeObjects.spot_roots (ConcreteMajor.spot_c r))
-          roots_out st cap /\
-        GenImpl.gen_gc_major_precondition
-          ConcreteMinor.spot_minor2
-          (ConcreteMajor.spot_major_heap r)
-          (ConcreteMajor.spot_major_fp r)
+          roots_out true st cap /\
+        GenImpl.gen_gc_stack_budget
           (ThreeObjects.spot_roots (ConcreteMajor.spot_c r))
           st cap)
       (ensures (
@@ -569,6 +555,7 @@ let prepared_roots_preserve_c_field1
   assert (U64.v (SpecObj.wosize_of_object c prepared_major) >= 2);
   ConcreteScenarios.spot_collection_heap_shape r;
   ConcreteScenarios.spot_roots_valid_for_minor_collection r;
+  ConcreteForwarding.spot_concrete_no_oom r;
   GenImpl.gen_gc_major_precondition_elim
     ConcreteMinor.spot_minor2
     (ConcreteMajor.spot_major_heap r)
@@ -671,12 +658,7 @@ let spot_concrete_c_field_final_points_to_a_prime
     st cap in
   assert (Seq.mem c prepared_roots);
   assert (Seq.mem a_prime prepared_roots);
-  assert (GenImpl.gen_gc_major_precondition
-    ConcreteMinor.spot_minor2
-    (ConcreteMajor.spot_major_heap r)
-    (ConcreteMajor.spot_major_fp r)
-    (ThreeObjects.spot_roots c)
-    st cap);
+  assert (GenImpl.gen_gc_stack_budget (ThreeObjects.spot_roots c) st cap);
   spot_root_heap_reachable_from_major_gc_pre r st cap c;
   spot_root_heap_reachable_from_major_gc_pre r st cap a_prime;
   assert (SpecCorrectness.major_gc_live_subgraph_isomorphism
