spot/GC.SPOT.CallFull.fst
@@ -52,14 +52,14 @@ fn call_gen_gc_spot
     pure (
       gen_gc_roots_post
         ({ data = 'd; bump = 'b } <: minor_state) 's 'fp 'rs
-        rs2 'st (stack_capacity st) /\
+        rs2 (snd res) 'st (stack_capacity st) /\
       gen_gc_heap_shape_post d2 b2 s2 /\
       gen_gc_reachable_subgraph_isomorphism_post
         ({ data = 'd; bump = 'b } <: minor_state) 's 'fp 'rs
         (snd res) s2 rs2 'st (stack_capacity st) /\
       gen_gc_unreachable_final_blue_post
         ({ data = 'd; bump = 'b } <: minor_state) 's 'fp 'rs
-        s2 'st (stack_capacity st))
+        (snd res) s2 'st (stack_capacity st))
 {
   Preconditions.gen_gc_pre_elim
     ({ data = 'd; bump = 'b } <: minor_state) 's 'fp 'rs 'farr 'sl
